Compiler/CompilationModel/ScopeValidation.lean
@@ -365,6 +365,8 @@ def validateScopedExprIdentifiers
     Expr.wMulDown a b => do
       validateScopedExprIdentifiers context params paramScope dynamicParams localScope constructorArgCount a
       validateScopedExprIdentifiers context params paramScope dynamicParams localScope constructorArgCount b
+  | Expr.intrinsic _ _ _ args =>
+      validateScopedExprIdentifiersList context params paramScope dynamicParams localScope constructorArgCount args
   | Expr.wDivUp a b => do
       validateArithDuplicatedOperandPurity context [b]
       validateScopedExprIdentifiers context params paramScope dynamicParams localScope constructorArgCount a
